work on encoding value relation

Proto.fst
@@ -1,6 +1,7 @@
 module Proto
 open FStar.UInt
 open FStar.Int.Cast.Full
+open FStar.Mul
 
 module U8 = FStar.UInt8
 module U16 = FStar.UInt16
@@ -44,7 +45,7 @@ type proto_enum_descriptor = {
   name : string;
   fields : list proto_enum_field;
 }
-and proto_enum_field = string * nat
+and proto_enum_field = string & nat
 
 unopteq
 type proto_msg_descriptor : Type = {
@@ -136,3 +137,78 @@ let proto_compat_field' (f1 f2 : proto_enc_field') : bool =
   | LEN' v1, LEN' v2 -> v1 = v2 
   | I32' v1, I32' v2 -> v1 = v2 
   | _, _ -> false)
+
+(* Beginning of comp and val relation *)
+
+(*
+   Compute x^n using exponentiation by squares.
+
+   For now, n must be positive. Since I have a few 
+   rules which require taking (-1)^n with a negative n,
+   we'll use the fact that (-1)^(-n) = (-1)^n. 
+
+   It seems tricky to get this function to do that since 
+   F* has to prove termination, so that trick will be applied 
+   in the relevant rule directly.
+*)
+let rec exp (x:int) (n:nat) : Tot int (decreases n) = 
+  if n = 0 then 
+    1
+  else if n % 2 = 0 then
+    exp (x * x) (n / 2)
+  else 
+    x * (exp (x * x) ((n - 1) / 2))
+
+let idn c = if c then 1 else 0
+
+let base = b:nat{b = 32 \/ b = 64}
+let uint_promote (v:int) : int = v
+let uint_demote (v:int) : int = v % pow2 32
+let int_promote (v:int) : int = v
+let int_demote' (v:int) : int = (v % pow2 32 - pow2 32 * (idn (v >= pow2 31))) % pow2 32
+let int_demote (v:int) : int = (v % pow2 32 - pow2 32 * (idn (v >= pow2 31))) % pow2 32
+let sint_promote (v:int) : int = v 
+let sint_demote (v:int) : int = v % pow2 31
+let uint_int (v:int) (b:base) : int = v - (pow2 b) * (idn (v >= pow2 (b - 1)))
+let int_uint (v:int) (b:base) : int = v + (pow2 b) * (idn (v < 0))
+let uint_sint (v:int) (b:base) : int = (exp (-1) (abs v)) * (v / 2) - (v % 2)
+let sint_uint (v:int) (b:base) : int = 2 * (abs v) - idn (v < 0)
+let int_sint (v:int) (b:base) : int = if v >= 0 then 
+    (exp (-1) (abs v)) * (v / 2) - (v % 2)
+  else 
+    (exp (-1) (abs v)) * (v + (pow2 (b - 1)) - (v / 2)) + (v % 2) 
+let sint_int (v:int) (b:base) : int = if -(pow2 (b-2)) <= v && v < pow2 (b-2) then 
+    2 * (abs v) - idn (v < 0) 
+  else 
+    abs (2 * v - pow2 (b-1)) - pow2 (b-1) - idn (v < pow2 (b-2))
+
+let val_rel (v1 : int) (t1 : proto_terminal) (v2 : int) (t2 : proto_terminal) = 
+  if t1 = t2 then 
+     v1 = v2 
+  else 
+  match t1, t2 with 
+  | STRING, BYTES 
+  | BYTES, STRING -> v1 = v2
+  | UINT32, UINT64 -> v2 = uint_promote v1
+  | UINT64, UINT64 -> v2 = uint_demote v1
+  | INT32, INT64 -> v2 = int_promote v1 
+  | INT64, INT32 -> v2 = int_demote v2 
+  | SINT32, SINT64 -> v2 = sint_promote v1
+  | SINT64, SINT32 -> v2 = sint_demote v1
+  | UINT32, INT32 -> v2 = uint_int v1 32
+  | UINT64, INT64 -> v2 = uint_int v2 64
+  | INT32, UINT32 -> v2 = int_uint v1 32
+  | INT64, UINT64 -> v2 = int_uint v2 64 
+  | UINT32, SINT32 -> v2 = uint_sint v1 32 
+  | UINT64, SINT64 -> v2 = uint_sint v1 64
+  | SINT32, UINT32 -> v2 = sint_uint v1 32 
+  | SINT64, UINT64 -> v2 = sint_uint v1 64
+  | INT32, SINT32 -> v2 = int_sint v1 32 
+  | INT64, SINT64 -> v2 = int_sint v1 64
+  | SINT32, INT32 -> v2 = sint_int v1 32 
+  | SINT64, INT64 -> v2 = sint_int v1 64
+  | _ -> false
+  
+let test = val_rel (-9) INT32 (-12) SINT32
+(* FIXME Off by one error from actual protobuf implementation *)
+let testv = int_sint (-9) 32
